Escallon/LR_Parsing/Item_Pushdown_Automata.thy
@@ -11,7 +11,7 @@ Possible solutions:
   2. Since state = top of stack: instead of state q and stack q#qs do state q and stack qs
       \<Longrightarrow> problems with empty stack? (IPDA accepts with final state)
 
-A definition with variant 2, using [S' \<rightarrow> [] . []] as a dummy starting stack symbol:
+A definition with variant 2, using [S' \<rightarrow> [] \<cdot> []] as a dummy starting stack symbol:
 *)
 
 print_record "(('n, 't) item, 't) npda"
@@ -19,15 +19,15 @@ print_record "(('n, 't) item, 't) npda"
 definition (in Extended_Cfg) IPDA :: "(('n, 't) item, 't) npda" where
   "IPDA \<equiv> let
     P = Prods G';
-    \<Delta> = {([[X \<rightarrow> \<beta> . Tm a # \<gamma>]], a, [[X \<rightarrow> \<beta> @ [Tm a] . \<gamma>]])|X \<beta> a \<gamma>. (X, \<beta> @ Tm a # \<gamma>) \<in> P};
-    \<E> = {([[X \<rightarrow> \<beta> . Nt Y # \<gamma>]], [[Y \<rightarrow> [] . \<alpha>], [X \<rightarrow> \<beta> . Nt Y # \<gamma>]])
+    \<Delta> = {([[X \<rightarrow> \<beta> \<cdot> Tm a # \<gamma>]], a, [[X \<rightarrow> \<beta> @ [Tm a] \<cdot> \<gamma>]])|X \<beta> a \<gamma>. (X, \<beta> @ Tm a # \<gamma>) \<in> P};
+    \<E> = {([[X \<rightarrow> \<beta> \<cdot> Nt Y # \<gamma>]], [[Y \<rightarrow> [] \<cdot> \<alpha>], [X \<rightarrow> \<beta> \<cdot> Nt Y # \<gamma>]])
         | X \<beta> Y \<gamma> \<alpha>. (X, \<beta> @ Nt Y # \<gamma>) \<in> P \<and> (Y, \<alpha>) \<in> P} \<union> 
-        {([[Y \<rightarrow> \<alpha> . []], [X \<rightarrow> \<beta> . Nt Y # \<gamma>]], [[X \<rightarrow> \<beta> @ [Nt Y] . \<gamma>]])
+        {([[Y \<rightarrow> \<alpha> \<cdot> []], [X \<rightarrow> \<beta> \<cdot> Nt Y # \<gamma>]], [[X \<rightarrow> \<beta> @ [Nt Y] \<cdot> \<gamma>]])
         | Y \<alpha> X \<beta> \<gamma>. (X, \<beta> @ Nt Y # \<gamma>) \<in> P \<and> (Y, \<alpha>) \<in> P}     
-  in \<lparr>npda.states = It G', init = [S' \<rightarrow> [] . [Nt S]], final = {[S' \<rightarrow> [Nt S] . []]}, nxt = \<Delta>, eps = \<E>\<rparr>"
+  in \<lparr>npda.states = It G', init = [S' \<rightarrow> [] \<cdot> [Nt S]], final = {[S' \<rightarrow> [Nt S] \<cdot> []]}, nxt = \<Delta>, eps = \<E>\<rparr>"
 
-(* \<lparr>init = [S' \<rightarrow> [] . [Nt S]], init_symbol = [S' \<rightarrow> [] . []], 
-      final = {[S' \<rightarrow> [Nt S] . []]}, nxt = \<Delta>, eps = \<E>\<rparr> *)
+(* \<lparr>init = [S' \<rightarrow> [] \<cdot> [Nt S]], init_symbol = [S' \<rightarrow> [] \<cdot> []], 
+      final = {[S' \<rightarrow> [Nt S] \<cdot> []]}, nxt = \<Delta>, eps = \<E>\<rparr> *)
 
 locale ipda = Extended_Cfg G for G :: "('n::fresh0, 't) Cfg" +
   fixes M :: "(('n, 't) item, 't) npda"
@@ -37,10 +37,10 @@ begin
 section \<open>Basic Properties\<close>
 
 lemma init_ipda [simp]:
-  "init M = [S' \<rightarrow> [] . [Nt S]]"
+  "init M = [S' \<rightarrow> [] \<cdot> [Nt S]]"
   using ipda unfolding IPDA_def by (meson npda.select_convs(2))
 
-abbreviation "final_state \<equiv> [S' \<rightarrow> [Nt S] . []]"
+abbreviation "final_state \<equiv> [S' \<rightarrow> [Nt S] \<cdot> []]"
 
 lemma final_ipda [simp]:
   "final M = {final_state}"
@@ -51,37 +51,37 @@ lemma final_state_in_It [simp]:
   unfolding It_defs G'_def by auto
 
 lemma nxt_ipda [simp]:
-  "nxt M = {([[X \<rightarrow> \<beta> . Tm a # \<gamma>]], a, [[X \<rightarrow> \<beta> @ [Tm a] . \<gamma>]])|X \<beta> a \<gamma>. (X, \<beta> @ Tm a # \<gamma>) \<in> Prods G'}"
+  "nxt M = {([[X \<rightarrow> \<beta> \<cdot> Tm a # \<gamma>]], a, [[X \<rightarrow> \<beta> @ [Tm a] \<cdot> \<gamma>]])|X \<beta> a \<gamma>. (X, \<beta> @ Tm a # \<gamma>) \<in> Prods G'}"
   using ipda unfolding IPDA_def by (meson select_convs(4))
 
 lemma nxt_Tm_neq_empty [simp]:
   assumes "a \<noteq> b"
-  shows "([X \<rightarrow> \<alpha> . Tm a # \<gamma>] # ps, b, q) \<notin> nxt M"
+  shows "([X \<rightarrow> \<alpha> \<cdot> Tm a # \<gamma>] # ps, b, q) \<notin> nxt M"
   using assms unfolding IPDA_def by simp
 
 lemma nxt_nempty_imp_Tm_eq:
   assumes "(ps, a, qs) \<in> nxt M"
-  obtains X \<beta> \<gamma> where "ps = [[X \<rightarrow> \<beta> . Tm a # \<gamma>]]" "(X, \<beta> @ Tm a # \<gamma>) \<in> Prods G'"
-    "qs = [[X \<rightarrow> \<beta> @ [Tm a] . \<gamma>]]"
+  obtains X \<beta> \<gamma> where "ps = [[X \<rightarrow> \<beta> \<cdot> Tm a # \<gamma>]]" "(X, \<beta> @ Tm a # \<gamma>) \<in> Prods G'"
+    "qs = [[X \<rightarrow> \<beta> @ [Tm a] \<cdot> \<gamma>]]"
   using assms by auto
 
 lemma nxt_nempty_imp_Tm_eq_Item:
-  assumes "([[X \<rightarrow> \<beta> . Tm a # \<gamma>]], b, q) \<in>  nxt M"
+  assumes "([[X \<rightarrow> \<beta> \<cdot> Tm a # \<gamma>]], b, q) \<in>  nxt M"
   shows "(X, \<beta> @ Tm a # \<gamma>) \<in> Prods G'" "a = b"
   using nxt_nempty_imp_Tm_eq[OF assms] by blast+
 
 lemma eps_ipda [simp]:
-  "eps M =  {([[X \<rightarrow> \<beta> . Nt Y # \<gamma>]], [Y \<rightarrow> [] . \<alpha>] # [[X \<rightarrow> \<beta> . Nt Y # \<gamma>]])
+  "eps M =  {([[X \<rightarrow> \<beta> \<cdot> Nt Y # \<gamma>]], [Y \<rightarrow> [] \<cdot> \<alpha>] # [[X \<rightarrow> \<beta> \<cdot> Nt Y # \<gamma>]])
         | X \<beta> Y \<gamma> \<alpha>. (X, \<beta> @ Nt Y # \<gamma>) \<in> Prods G' \<and> (Y, \<alpha>) \<in> Prods G'} \<union> 
-        {([[Y \<rightarrow> \<alpha> . []], [X \<rightarrow> \<beta> . Nt Y # \<gamma>]], [[X \<rightarrow> \<beta> @ [Nt Y] . \<gamma>]])
+        {([[Y \<rightarrow> \<alpha> \<cdot> []], [X \<rightarrow> \<beta> \<cdot> Nt Y # \<gamma>]], [[X \<rightarrow> \<beta> @ [Nt Y] \<cdot> \<gamma>]])
         | Y \<alpha> X \<beta> \<gamma>. (X, \<beta> @ Nt Y # \<gamma>) \<in> Prods G' \<and> (Y, \<alpha>) \<in> Prods G'}"
   using ipda unfolding IPDA_def by (meson select_convs(5))
 
 lemma eps_cases [consumes 1, case_names expand reduce]:
   assumes "(ps, qs) \<in> eps M" 
-  obtains X \<beta> Y \<gamma> \<alpha> where "ps = [[X \<rightarrow> \<beta> . Nt Y # \<gamma>]]" "qs = [[Y \<rightarrow> [] . \<alpha>], [X \<rightarrow> \<beta> . Nt Y # \<gamma>]]"
+  obtains X \<beta> Y \<gamma> \<alpha> where "ps = [[X \<rightarrow> \<beta> \<cdot> Nt Y # \<gamma>]]" "qs = [[Y \<rightarrow> [] \<cdot> \<alpha>], [X \<rightarrow> \<beta> \<cdot> Nt Y # \<gamma>]]"
     "(X, \<beta> @ Nt Y # \<gamma>) \<in> Prods G'" "(Y, \<alpha>) \<in> Prods G'" |
-    Y \<alpha> X \<beta> \<gamma> where "ps = [[Y \<rightarrow> \<alpha> . []], [X \<rightarrow> \<beta> . Nt Y # \<gamma>]]" "qs =  [[X \<rightarrow> \<beta> @ [Nt Y] . \<gamma>]]"
+    Y \<alpha> X \<beta> \<gamma> where "ps = [[Y \<rightarrow> \<alpha> \<cdot> []], [X \<rightarrow> \<beta> \<cdot> Nt Y # \<gamma>]]" "qs =  [[X \<rightarrow> \<beta> @ [Nt Y] \<cdot> \<gamma>]]"
      "(X, \<beta> @ Nt Y # \<gamma>) \<in> Prods G'" "(Y, \<alpha>) \<in> Prods G'"
   using assms unfolding eps_ipda by auto
 
@@ -118,9 +118,9 @@ lemma step_len_dec:
 
 lemma shifting [simp]:
   assumes "(A, \<alpha> @ Tm a # \<beta>) \<in> Prods G'"
-  shows "([A \<rightarrow> \<alpha> . Tm a # \<beta>]#\<rho>s, a#u) \<turnstile> ([A \<rightarrow> \<alpha>@[Tm a] . \<beta>]#\<rho>s, u)"
+  shows "([A \<rightarrow> \<alpha> \<cdot> Tm a # \<beta>]#\<rho>s, a#u) \<turnstile> ([A \<rightarrow> \<alpha>@[Tm a] \<cdot> \<beta>]#\<rho>s, u)"
 proof -
-  have "([[A \<rightarrow> \<alpha> . Tm a # \<beta>]], a, [[A \<rightarrow> \<alpha> @ [Tm a] . \<beta>]]) \<in> nxt M"
+  have "([[A \<rightarrow> \<alpha> \<cdot> Tm a # \<beta>]], a, [[A \<rightarrow> \<alpha> @ [Tm a] \<cdot> \<beta>]]) \<in> nxt M"
     using IPDA_def assms by auto
   then show ?thesis using step_nxt 
     by (metis Cons_eq_appendI append.left_neutral)
@@ -128,40 +128,40 @@ qed
 
 lemma reducing [simp]:
   assumes "(Y, \<alpha>) \<in> Prods G'" "(X, \<beta> @ Nt Y # \<gamma>) \<in> Prods G'"
-  shows "([Y \<rightarrow> \<alpha> . []]#[X \<rightarrow> \<beta> . Nt Y#\<gamma>]#\<rho>, w) \<turnstile> ([X \<rightarrow> \<beta> @ [Nt Y] . \<gamma>]#\<rho>, w)"
+  shows "([Y \<rightarrow> \<alpha> \<cdot> []]#[X \<rightarrow> \<beta> \<cdot> Nt Y#\<gamma>]#\<rho>, w) \<turnstile> ([X \<rightarrow> \<beta> @ [Nt Y] \<cdot> \<gamma>]#\<rho>, w)"
 proof -
-  have "([[Y \<rightarrow> \<alpha> . []], [X \<rightarrow> \<beta> . Nt Y#\<gamma>]] @ \<rho>, w) \<turnstile> ([[X \<rightarrow> \<beta> @ [Nt Y] . \<gamma>]] @ \<rho>, w)"
+  have "([[Y \<rightarrow> \<alpha> \<cdot> []], [X \<rightarrow> \<beta> \<cdot> Nt Y#\<gamma>]] @ \<rho>, w) \<turnstile> ([[X \<rightarrow> \<beta> @ [Nt Y] \<cdot> \<gamma>]] @ \<rho>, w)"
     by (rule step_eps) (use assms in fastforce)
   thus ?thesis by simp
 qed
 
 lemma expanding_in_eps:
   assumes "(Y, \<alpha>) \<in> Prods G'" "(X, \<beta> @ Nt Y # \<gamma>) \<in> Prods G'" 
-  shows "([[X \<rightarrow> \<beta> . Nt Y#\<gamma>]], [[Y \<rightarrow> [] . \<alpha>], [X \<rightarrow> \<beta> . Nt Y#\<gamma>]]) \<in> eps M"
+  shows "([[X \<rightarrow> \<beta> \<cdot> Nt Y#\<gamma>]], [[Y \<rightarrow> [] \<cdot> \<alpha>], [X \<rightarrow> \<beta> \<cdot> Nt Y#\<gamma>]]) \<in> eps M"
   using assms by auto
 
 lemma expanding:
   assumes "(Y, \<alpha>) \<in> Prods G'" "(X, \<beta> @ Nt Y # \<gamma>) \<in> Prods G'"
-  shows "([X \<rightarrow> \<beta> . Nt Y#\<gamma>]#\<rho>, w) \<turnstile> ([Y \<rightarrow> [] . \<alpha>]#[X \<rightarrow> \<beta> . Nt Y#\<gamma>]#\<rho>, w)"
+  shows "([X \<rightarrow> \<beta> \<cdot> Nt Y#\<gamma>]#\<rho>, w) \<turnstile> ([Y \<rightarrow> [] \<cdot> \<alpha>]#[X \<rightarrow> \<beta> \<cdot> Nt Y#\<gamma>]#\<rho>, w)"
 proof -
-  have "([[X \<rightarrow> \<beta> . Nt Y#\<gamma>]] @ \<rho>, w) \<turnstile> ([[Y \<rightarrow> [] . \<alpha>], [X \<rightarrow> \<beta> . Nt Y#\<gamma>]] @ \<rho>, w)"
+  have "([[X \<rightarrow> \<beta> \<cdot> Nt Y#\<gamma>]] @ \<rho>, w) \<turnstile> ([[Y \<rightarrow> [] \<cdot> \<alpha>], [X \<rightarrow> \<beta> \<cdot> Nt Y#\<gamma>]] @ \<rho>, w)"
     using assms by fastforce
   thus ?thesis by simp
 qed
 
 lemma expanding_singleton:
   assumes "Prods G' \<turnstile> [Nt Y] \<Rightarrow> \<alpha>" "(X, \<beta> @ Nt Y # \<gamma>) \<in> Prods G'"
-  shows "([X \<rightarrow> \<beta> . Nt Y#\<gamma>]#\<rho>, w) \<turnstile> ([Y \<rightarrow> [] . \<alpha>]#[X \<rightarrow> \<beta> . Nt Y#\<gamma>]#\<rho>, w)"
+  shows "([X \<rightarrow> \<beta> \<cdot> Nt Y#\<gamma>]#\<rho>, w) \<turnstile> ([Y \<rightarrow> [] \<cdot> \<alpha>]#[X \<rightarrow> \<beta> \<cdot> Nt Y#\<gamma>]#\<rho>, w)"
   using assms expanding by (simp add: derive_singleton)
 
 lemma step_cases[consumes 1, case_names shift reduce expand, cases set: step]:
   assumes "c0 \<turnstile> c1"
 obtains A \<alpha> a \<beta> \<rho> u where 
-    "c0 = ([A \<rightarrow> \<alpha> . Tm a # \<beta>]#\<rho>, a#u)" "c1 = ([A \<rightarrow> \<alpha>@[Tm a] . \<beta>]#\<rho>, u)" |
+    "c0 = ([A \<rightarrow> \<alpha> \<cdot> Tm a # \<beta>]#\<rho>, a#u)" "c1 = ([A \<rightarrow> \<alpha>@[Tm a] \<cdot> \<beta>]#\<rho>, u)" |
     Y \<alpha> X \<beta> \<gamma> \<rho> w where
-      "c0 = ([Y \<rightarrow> \<alpha> . []]#[X \<rightarrow> \<beta> . Nt Y#\<gamma>]#\<rho>, w)"  "c1 = ([X \<rightarrow> \<beta> @ [Nt Y] . \<gamma>]#\<rho>, w)" |
+      "c0 = ([Y \<rightarrow> \<alpha> \<cdot> []]#[X \<rightarrow> \<beta> \<cdot> Nt Y#\<gamma>]#\<rho>, w)"  "c1 = ([X \<rightarrow> \<beta> @ [Nt Y] \<cdot> \<gamma>]#\<rho>, w)" |
     Y \<alpha> X \<beta> \<gamma> \<rho> w where 
-    "c0 = ([X \<rightarrow> \<beta> . Nt Y#\<gamma>]#\<rho>, w)"  "c1 = ([Y \<rightarrow> [] . \<alpha>]#[X \<rightarrow> \<beta> . Nt Y#\<gamma>]#\<rho>, w)"
+    "c0 = ([X \<rightarrow> \<beta> \<cdot> Nt Y#\<gamma>]#\<rho>, w)"  "c1 = ([Y \<rightarrow> [] \<cdot> \<alpha>]#[X \<rightarrow> \<beta> \<cdot> Nt Y#\<gamma>]#\<rho>, w)"
   using assms by cases auto
 
 lemma step_imp_in_Prods:
@@ -180,7 +180,7 @@ lemma step_imp_not_Nil:
   using assms by cases auto
 
 lemma expanding_imp_in_Prods_G:
-  assumes "([X \<rightarrow> \<alpha> . Nt Y # \<beta>] # \<rho>, u) \<turnstile> ([Y \<rightarrow> [] . \<gamma>] # [X \<rightarrow> \<alpha> . Nt Y # \<beta>] # \<rho>, v)"
+  assumes "([X \<rightarrow> \<alpha> \<cdot> Nt Y # \<beta>] # \<rho>, u) \<turnstile> ([Y \<rightarrow> [] \<cdot> \<gamma>] # [X \<rightarrow> \<alpha> \<cdot> Nt Y # \<beta>] # \<rho>, v)"
   shows "(Y, \<gamma>) \<in> Prods G"
 proof -
   from assms have "(Y, \<gamma>) \<in> Prods G'" using step_imp_in_Prods by fastforce
@@ -195,14 +195,14 @@ qed
 
 lemma step_not_expanding_unique:
   assumes "(\<rho>, u) \<turnstile> c0" "(\<rho>, u) \<turnstile> c1"
-    "\<exists>X \<alpha> a \<beta>. hd \<rho> = [X \<rightarrow> \<alpha> . []] \<or> hd \<rho> = [X \<rightarrow> \<alpha> . Tm a # \<beta>]"
+    "\<exists>X \<alpha> a \<beta>. hd \<rho> = [X \<rightarrow> \<alpha> \<cdot> []] \<or> hd \<rho> = [X \<rightarrow> \<alpha> \<cdot> Tm a # \<beta>]"
   shows "c0 = c1"
   using assms(1) by (cases; use assms(2) in cases, use assms(3) in auto)
 
 
 lemma step_reaches_final_imp_S:
-  assumes "([A \<rightarrow> \<alpha> . \<beta>] # \<rho> @ \<sigma>, u) \<turnstile> (final_state # \<sigma>, v)"
-  shows "([A \<rightarrow> \<alpha> . \<beta>] # \<rho> @ \<sigma>, u) = ([S \<rightarrow> \<alpha> . \<beta>] # init M # \<sigma>, v)"
+  assumes "([A \<rightarrow> \<alpha> \<cdot> \<beta>] # \<rho> @ \<sigma>, u) \<turnstile> (final_state # \<sigma>, v)"
+  shows "([A \<rightarrow> \<alpha> \<cdot> \<beta>] # \<rho> @ \<sigma>, u) = ([S \<rightarrow> \<alpha> \<cdot> \<beta>] # init M # \<sigma>, v)"
   using assms(1) by cases auto
 
 
@@ -216,13 +216,13 @@ abbreviation stepn ( \<open>_ \<turnstile>'(_') _\<close> 50) where
 
 lemma step_not_expanding_imp_reaches:
   assumes "(\<rho>, u) \<turnstile> c0" "(\<rho>, u) \<turnstile>(Suc n) c1"
-    "\<exists>X \<alpha> a \<beta>. hd \<rho> = [X \<rightarrow> \<alpha> . []] \<or> hd \<rho> = [X \<rightarrow> \<alpha> . Tm a # \<beta>]"
+    "\<exists>X \<alpha> a \<beta>. hd \<rho> = [X \<rightarrow> \<alpha> \<cdot> []] \<or> hd \<rho> = [X \<rightarrow> \<alpha> \<cdot> Tm a # \<beta>]"
   shows "c0 \<turnstile>(n) c1"
   using step_not_expanding_unique assms by (metis relpowp_Suc_D2)
 
 lemma stepn_neq_imp_not_expanding_reaches:
   assumes "(\<rho>, u) \<turnstile> c0" "(\<rho>, u) \<turnstile>(n) c1" "(\<rho>, u) \<noteq> c1"
-    "\<exists>X \<alpha> a \<beta>. hd \<rho> = [X \<rightarrow> \<alpha> . []] \<or> hd \<rho> = [X \<rightarrow> \<alpha> . Tm a # \<beta>]"
+    "\<exists>X \<alpha> a \<beta>. hd \<rho> = [X \<rightarrow> \<alpha> \<cdot> []] \<or> hd \<rho> = [X \<rightarrow> \<alpha> \<cdot> Tm a # \<beta>]"
   obtains m where "n = Suc m" "c0 \<turnstile>(m) c1"
   using assms step_not_expanding_imp_reaches by (metis relpowp_E2)
 
@@ -234,11 +234,11 @@ lemma steps_len_dec:
 
 lemma completes_Tms:
   "(A, \<alpha> @ map Tm u @ \<beta>) \<in> Prods G' 
-    \<Longrightarrow> ([A \<rightarrow> \<alpha> . map Tm u @ \<beta>]#is, u@v) \<turnstile>* ([A \<rightarrow> \<alpha> @ map Tm u . \<beta>]#is, v)"
+    \<Longrightarrow> ([A \<rightarrow> \<alpha> \<cdot> map Tm u @ \<beta>]#is, u@v) \<turnstile>* ([A \<rightarrow> \<alpha> @ map Tm u \<cdot> \<beta>]#is, v)"
 proof (induction u arbitrary: \<alpha>)
   case (Cons a u)
-  hence "([A \<rightarrow> \<alpha> . map Tm (a # u) @ \<beta>] #  is, (a # u) @ v) 
-        \<turnstile> ([A \<rightarrow> \<alpha> @ [Tm a] . map Tm u @ \<beta>] # is, u @ v)"
+  hence "([A \<rightarrow> \<alpha> \<cdot> map Tm (a # u) @ \<beta>] #  is, (a # u) @ v) 
+        \<turnstile> ([A \<rightarrow> \<alpha> @ [Tm a] \<cdot> map Tm u @ \<beta>] # is, u @ v)"
     by simp
   also note Cons(1)[of "\<alpha>@[Tm a]"] 
   finally show ?case using Cons by auto
@@ -301,14 +301,14 @@ lemma reachable_imp_substring:
 qed simp
 
 corollary steps_shift_decomp:
-  assumes "(\<rho>, u @ v) \<turnstile>* ([A \<rightarrow> \<alpha> . Tm a # \<beta>] # \<sigma>, a # v)"
-    "([A \<rightarrow> \<alpha> . Tm a # \<beta>] # \<sigma>, a # v) \<turnstile> (\<tau>, v)"
+  assumes "(\<rho>, u @ v) \<turnstile>* ([A \<rightarrow> \<alpha> \<cdot> Tm a # \<beta>] # \<sigma>, a # v)"
+    "([A \<rightarrow> \<alpha> \<cdot> Tm a # \<beta>] # \<sigma>, a # v) \<turnstile> (\<tau>, v)"
   obtains x where "u = x @ [a]"
   using reachable_imp_substring[OF assms(1)] by auto
 
 lemma init_expands[elim]:
   assumes "(init M # \<rho>, u) \<turnstile> (\<sigma>, v)"
-  obtains \<alpha> where "(\<sigma>, v) = ([S \<rightarrow> [] . \<alpha>] # init M # \<rho>, u)"
+  obtains \<alpha> where "(\<sigma>, v) = ([S \<rightarrow> [] \<cdot> \<alpha>] # init M # \<rho>, u)"
     "(S, \<alpha>) \<in> Prods G"
   using assms proof cases
   case (expand Y \<alpha> X \<beta> \<gamma> \<rho> w)
@@ -317,30 +317,30 @@ lemma init_expands[elim]:
 qed auto
 
 lemma complete_S'_step_impossible:
-  assumes "([S' \<rightarrow> \<alpha> . []] # \<rho>, w) \<turnstile> c"
+  assumes "([S' \<rightarrow> \<alpha> \<cdot> []] # \<rho>, w) \<turnstile> c"
   shows False
   using assms S'_Prod_notin_G' assms step_imp_in_Prods by cases force+
 
 lemma second_notin_It_imp_complete_step_impossible:
-  assumes "([A \<rightarrow> \<alpha> . []] # i # \<rho>, w) \<turnstile> c"
+  assumes "([A \<rightarrow> \<alpha> \<cdot> []] # i # \<rho>, w) \<turnstile> c"
     "i \<notin> It G'"
   shows False
   using assms proof cases
   case (reduce Y \<alpha> X \<beta> \<gamma> \<rho> w)
   then show False using assms 
-      prod_of_item_eq_imp_in_Prods_eq[of "[X \<rightarrow> \<beta> . Nt Y # \<gamma>]" "[X \<rightarrow> \<beta> @ [Nt Y] . \<gamma>]"] 
+      prod_of_item_eq_imp_in_Prods_eq[of "[X \<rightarrow> \<beta> \<cdot> Nt Y # \<gamma>]" "[X \<rightarrow> \<beta> @ [Nt Y] \<cdot> \<gamma>]"] 
       step_imp_in_It by auto
 qed simp_all
 
 lemma complete_S'_steps_refl:
-  assumes "([[S' \<rightarrow> \<alpha> . []]], w) \<turnstile>* c"
-  shows "([[S' \<rightarrow> \<alpha> . []]], w) = c"
+  assumes "([[S' \<rightarrow> \<alpha> \<cdot> []]], w) \<turnstile>* c"
+  shows "([[S' \<rightarrow> \<alpha> \<cdot> []]], w) = c"
   using assms complete_S'_step_impossible by (cases rule: converse_rtranclpE) blast+
 
 lemma reachable_imp_init_or_in_G:
   assumes "([init M], u) \<turnstile>* (\<rho>, v)"
-  obtains \<sigma> \<alpha> \<beta> where "\<rho> = \<sigma> @ [[S' \<rightarrow> \<alpha> . \<beta>]]" "\<alpha> @ \<beta> = [Nt S]"
-    "\<forall>i \<in> set \<sigma>. case i of [X \<rightarrow> \<gamma> . \<delta>] \<Rightarrow> (X, \<gamma>@\<delta>) \<in> Prods G"
+  obtains \<sigma> \<alpha> \<beta> where "\<rho> = \<sigma> @ [[S' \<rightarrow> \<alpha> \<cdot> \<beta>]]" "\<alpha> @ \<beta> = [Nt S]"
+    "\<forall>i \<in> set \<sigma>. case i of [X \<rightarrow> \<gamma> \<cdot> \<delta>] \<Rightarrow> (X, \<gamma>@\<delta>) \<in> Prods G"
 proof -
   from assms obtain n where "([init M], u) \<turnstile>(n) (\<rho>, v)"
     using rtranclp_imp_relpowp by fast
@@ -352,8 +352,8 @@ proof -
     then obtain \<sigma> w where n_steps: "([init M], u) \<turnstile>(n) (\<sigma>, w)" 
       "(\<sigma>, w) \<turnstile> (\<rho>, v)" by auto
     from Suc.IH[OF this(1)] obtain \<tau> \<alpha> \<beta> where \<tau>_def:
-      "\<sigma> = \<tau> @ [[S' \<rightarrow> \<alpha> . \<beta>]]" "\<alpha> @ \<beta> = [Nt S]" 
-      "\<forall>i \<in> set \<tau>. case i of [X \<rightarrow> \<gamma> . \<delta>] \<Rightarrow> (X, \<gamma>@\<delta>) \<in> Prods G" (is "\<forall>i \<in> _. ?in_Prods i")
+      "\<sigma> = \<tau> @ [[S' \<rightarrow> \<alpha> \<cdot> \<beta>]]" "\<alpha> @ \<beta> = [Nt S]" 
+      "\<forall>i \<in> set \<tau>. case i of [X \<rightarrow> \<gamma> \<cdot> \<delta>] \<Rightarrow> (X, \<gamma>@\<delta>) \<in> Prods G" (is "\<forall>i \<in> _. ?in_Prods i")
       by blast
     from n_steps(2) show ?case 
     proof (cases \<tau>)
@@ -364,13 +364,13 @@ proof -
         using Suc.prems(2)[of _ "[]" "[Nt S]"] \<sigma>_init by force
     next
       case (Cons i \<upsilon>)
-      hence \<sigma>_def: "\<sigma> = i # \<upsilon> @ [[S' \<rightarrow> \<alpha> . \<beta>]]" using \<tau>_def by simp
+      hence \<sigma>_def: "\<sigma> = i # \<upsilon> @ [[S' \<rightarrow> \<alpha> \<cdot> \<beta>]]" using \<tau>_def by simp
       from n_steps(2)[unfolded this] show ?thesis 
       proof cases
         case (expand Y \<alpha>' X \<beta>' \<gamma> \<rho>' w')
         moreover with Cons have
-          "\<rho> = [Y \<rightarrow> [] . \<alpha>'] # \<tau> @ [[S' \<rightarrow> \<alpha> . \<beta>]]" by simp
-        moreover from expand \<tau>_def Cons have "\<forall>i\<in>set ([Y \<rightarrow> [] . \<alpha>'] # \<tau>). ?in_Prods i" 
+          "\<rho> = [Y \<rightarrow> [] \<cdot> \<alpha>'] # \<tau> @ [[S' \<rightarrow> \<alpha> \<cdot> \<beta>]]" by simp
+        moreover from expand \<tau>_def Cons have "\<forall>i\<in>set ([Y \<rightarrow> [] \<cdot> \<alpha>'] # \<tau>). ?in_Prods i" 
           using \<sigma>_def  expanding_imp_in_Prods_G expand n_steps(2) \<tau>_def(3) by auto
         ultimately show ?thesis using Suc.prems(2) \<tau>_def Cons by fastforce
       qed (cases \<upsilon>, (use \<tau>_def Cons Suc in auto))+
@@ -381,8 +381,8 @@ qed
 lemma first_step_is_eps:
   assumes "([init M], u) \<turnstile>(Suc n) (qs, v)"
   obtains \<alpha> where 
-    "([init M], u) \<turnstile> ([[S \<rightarrow> [] . \<alpha>], init M], u)"
-    "([[S \<rightarrow> [] . \<alpha>], init M], u) \<turnstile>* (qs, v)"
+    "([init M], u) \<turnstile> ([[S \<rightarrow> [] \<cdot> \<alpha>], init M], u)"
+    "([[S \<rightarrow> [] \<cdot> \<alpha>], init M], u) \<turnstile>* (qs, v)"
 proof -
   from assms obtain ps u' where step: "([init M], u) \<turnstile> (ps, u')"
     and steps: "(ps, u') \<turnstile>* (qs, v)"
@@ -394,13 +394,13 @@ proof -
 qed
 
 lemma reachable_snd_not_empty_imp_hd_in_G:
-  assumes "([init M], u) \<turnstile>* ([A \<rightarrow> \<alpha> . \<beta>] # [B \<rightarrow> \<gamma> . \<delta>] # \<rho>, v)"
+  assumes "([init M], u) \<turnstile>* ([A \<rightarrow> \<alpha> \<cdot> \<beta>] # [B \<rightarrow> \<gamma> \<cdot> \<delta>] # \<rho>, v)"
     "\<gamma>@\<delta> \<noteq> []"
   shows "(A, \<alpha>@\<beta>) \<in> Prods G"
 proof -
   from reachable_imp_init_or_in_G[OF assms(1)] obtain \<sigma> \<alpha>' \<beta>' where \<sigma>_def:
-    "[A \<rightarrow> \<alpha> . \<beta>] # [B \<rightarrow> \<gamma> . \<delta>] # \<rho> = \<sigma> @ [[S' \<rightarrow> \<alpha>' . \<beta>']]" "\<alpha>' @ \<beta>' = [Nt S]"
-    "\<forall>i\<in>set \<sigma>. case i of [X \<rightarrow> \<gamma> . \<delta>] \<Rightarrow> (X, \<gamma> @ \<delta>) \<in> Prods G"
+    "[A \<rightarrow> \<alpha> \<cdot> \<beta>] # [B \<rightarrow> \<gamma> \<cdot> \<delta>] # \<rho> = \<sigma> @ [[S' \<rightarrow> \<alpha>' \<cdot> \<beta>']]" "\<alpha>' @ \<beta>' = [Nt S]"
+    "\<forall>i\<in>set \<sigma>. case i of [X \<rightarrow> \<gamma> \<cdot> \<delta>] \<Rightarrow> (X, \<gamma> @ \<delta>) \<in> Prods G"
     by blast
   have "\<sigma> \<noteq> []" 
     by standard (use assms(2) \<sigma>_def in auto)
@@ -411,18 +411,18 @@ qed
 lemma singleton_derive_imp_completes:
   assumes "Prods G' \<turnstile> [Nt X] \<Rightarrow> map Tm u"
     "(A, \<alpha> @ Nt X # \<beta>) \<in> Prods G'"
-  shows "([A \<rightarrow> \<alpha> . [Nt X] @ \<beta>] # \<rho>, u @ v) 
-          \<turnstile>* ([A \<rightarrow> \<alpha> @ [Nt X] . \<beta>] # \<rho>, v)"
+  shows "([A \<rightarrow> \<alpha> \<cdot> [Nt X] @ \<beta>] # \<rho>, u @ v) 
+          \<turnstile>* ([A \<rightarrow> \<alpha> @ [Nt X] \<cdot> \<beta>] # \<rho>, v)"
 proof -
   note deriv = derive_singleton[of "Prods G'" "Nt X" "map Tm u"]
   with assms expanding have 
-    "([A \<rightarrow> \<alpha> . [Nt X] @ \<beta>] # \<rho>, u @ v) 
-      \<turnstile> ([X \<rightarrow> [] . map Tm u] # [A \<rightarrow> \<alpha> . [Nt X] @ \<beta>] # \<rho>, u @ v)"
+    "([A \<rightarrow> \<alpha> \<cdot> [Nt X] @ \<beta>] # \<rho>, u @ v) 
+      \<turnstile> ([X \<rightarrow> [] \<cdot> map Tm u] # [A \<rightarrow> \<alpha> \<cdot> [Nt X] @ \<beta>] # \<rho>, u @ v)"
     by auto
   also with completes_Tms step_imp_in_Prods have 
-    "... \<turnstile>* ([X \<rightarrow> map Tm u . []] # [A \<rightarrow> \<alpha> . [Nt X] @ \<beta>] # \<rho>, v)" 
+    "... \<turnstile>* ([X \<rightarrow> map Tm u \<cdot> []] # [A \<rightarrow> \<alpha> \<cdot> [Nt X] @ \<beta>] # \<rho>, v)" 
     by (metis deriv append.right_neutral append_Nil assms(1) completes_Tms sym.inject(1))
-  also  have "... \<turnstile> ([A \<rightarrow> \<alpha> @ [Nt X] . \<beta>] # \<rho>, v)"
+  also  have "... \<turnstile> ([A \<rightarrow> \<alpha> @ [Nt X] \<cdot> \<beta>] # \<rho>, v)"
     using assms deriv by auto
   finally show ?thesis .
 qed
@@ -432,18 +432,18 @@ section \<open>Language Equivalence\<close>
 lemma derive_imp_completes:
   assumes "Prods G' \<turnstile> \<beta> \<Rightarrow> map Tm w"
     "(A, \<alpha> @ \<beta> @ \<gamma>) \<in> Prods G'"
-  shows "([A \<rightarrow> \<alpha> . \<beta>@\<gamma>] # \<rho>, w @ x) \<turnstile>* ([A \<rightarrow> \<alpha>@\<beta> . \<gamma>] # \<rho>, x)"
+  shows "([A \<rightarrow> \<alpha> \<cdot> \<beta>@\<gamma>] # \<rho>, w @ x) \<turnstile>* ([A \<rightarrow> \<alpha>@\<beta> \<cdot> \<gamma>] # \<rho>, x)"
 proof -
   from derive_word_imp_single_Nt[OF assms(1)] obtain u v X y where \<beta>_decomp:
     "\<beta> = map Tm u @ Nt X # map Tm y" "Prods G' \<turnstile> [Nt X] \<Rightarrow> map Tm v" "w = u @ v @ y" by metis
   with completes_Tms[of A \<alpha> u "Nt X # map Tm y @ \<gamma>" _ "v @ y @ x"] have 
-    "([A \<rightarrow> \<alpha> . \<beta> @ \<gamma>] # \<rho>, w @ x) 
-      \<turnstile>* ([A \<rightarrow> \<alpha> @ map Tm u . Nt X # map Tm y @ \<gamma>] # \<rho>, v @ y @ x)" 
+    "([A \<rightarrow> \<alpha> \<cdot> \<beta> @ \<gamma>] # \<rho>, w @ x) 
+      \<turnstile>* ([A \<rightarrow> \<alpha> @ map Tm u \<cdot> Nt X # map Tm y @ \<gamma>] # \<rho>, v @ y @ x)" 
     using assms by simp
   also from singleton_derive_imp_completes[OF \<beta>_decomp(2), of _ "\<alpha> @ map Tm u" _ _ "y@x"] have 
-    "... \<turnstile>* ([A \<rightarrow> \<alpha> @ map Tm u @ [Nt X] . map Tm y @ \<gamma>] # \<rho>, y @ x)"
+    "... \<turnstile>* ([A \<rightarrow> \<alpha> @ map Tm u @ [Nt X] \<cdot> map Tm y @ \<gamma>] # \<rho>, y @ x)"
     using \<beta>_decomp(1) assms(2) by auto
-  also from completes_Tms have "... \<turnstile>* ([A \<rightarrow> \<alpha> @ \<beta> . \<gamma>] # \<rho>, x)"
+  also from completes_Tms have "... \<turnstile>* ([A \<rightarrow> \<alpha> @ \<beta> \<cdot> \<gamma>] # \<rho>, x)"
     using \<beta>_decomp by (smt (verit) append.assoc append_Cons append_Nil assms(2))
   finally show ?thesis .
 qed
@@ -452,7 +452,7 @@ qed
 lemma derives_imp_completes:
   assumes "Prods G' \<turnstile> \<beta> \<Rightarrow>* map Tm w"
     "(A, \<alpha> @ \<beta> @ \<gamma>) \<in> Prods G'"
-  shows "([A \<rightarrow> \<alpha> . \<beta>@\<gamma>] # \<rho>, w @ x) \<turnstile>* ([A \<rightarrow> \<alpha>@\<beta> . \<gamma>] # \<rho>, x)"
+  shows "([A \<rightarrow> \<alpha> \<cdot> \<beta>@\<gamma>] # \<rho>, w @ x) \<turnstile>* ([A \<rightarrow> \<alpha>@\<beta> \<cdot> \<gamma>] # \<rho>, x)"
 proof -
   from assms obtain n where "Prods G' \<turnstile> \<beta> \<Rightarrow>(n) map Tm w" 
     using rtranclp_imp_relpowp by fast
@@ -470,13 +470,13 @@ proof -
         "w = u @ v @ y" "i + j + k = n" "j > 0" 
         using less(3)  by (smt (verit, best))
       hence leqs: "i < n" "k < n" by auto
-      have first: "([A \<rightarrow> \<alpha> . \<beta> @ \<gamma>] # \<rho>, w @ x) 
-              \<turnstile>* ([A \<rightarrow> \<alpha> @ \<delta>\<^sub>1 . Nt X # \<delta>\<^sub>2 @ \<gamma>] # \<rho>, v @ y @ x)"
+      have first: "([A \<rightarrow> \<alpha> \<cdot> \<beta> @ \<gamma>] # \<rho>, w @ x) 
+              \<turnstile>* ([A \<rightarrow> \<alpha> @ \<delta>\<^sub>1 \<cdot> Nt X # \<delta>\<^sub>2 @ \<gamma>] # \<rho>, v @ y @ x)"
         (is "_ \<turnstile>* (?\<sigma>, _)")
         using less(1)[OF leqs(1) _ \<beta>_decomp(2), of _ _ "Nt X # \<delta>\<^sub>2 @ \<gamma>" _ "v @ y @ x"]
           \<beta>_decomp less.prems(1) by simp
-      have last: "([A \<rightarrow> \<alpha> @ \<delta>\<^sub>1 @ [Nt X] . \<delta>\<^sub>2 @ \<gamma>] # \<rho>, y @ x) 
-                  \<turnstile>* ([A \<rightarrow> \<alpha> @ \<beta> . \<gamma>] # \<rho>, x)"
+      have last: "([A \<rightarrow> \<alpha> @ \<delta>\<^sub>1 @ [Nt X] \<cdot> \<delta>\<^sub>2 @ \<gamma>] # \<rho>, y @ x) 
+                  \<turnstile>* ([A \<rightarrow> \<alpha> @ \<beta> \<cdot> \<gamma>] # \<rho>, x)"
         using less(1)[OF leqs(2) _ \<beta>_decomp(4), of _ "\<alpha> @ \<delta>\<^sub>1 @ [Nt X]"] \<beta>_decomp(1) less.prems(1) by simp
       show ?thesis 
       proof (cases "j = n")
@@ -502,26 +502,26 @@ proof -
           hence Y_prod': "(Y, \<gamma>') \<in> Prods G'" using derive_singleton 
             by (metis sym.inject(1))
           from m_steps \<beta>'_decomp(1) have X_step: "(X, \<xi>\<^sub>1 @ Nt Y # \<xi>\<^sub>2) \<in> Prods G'" 
-            "([A \<rightarrow> \<alpha> @ \<delta>\<^sub>1 . Nt X # \<delta>\<^sub>2 @ \<gamma>] # \<rho>, v @ y @ x) 
-              \<turnstile> ([X \<rightarrow> [] . \<xi>\<^sub>1 @ Nt Y # \<xi>\<^sub>2] # ?\<sigma>, v @ y @ x)" 
+            "([A \<rightarrow> \<alpha> @ \<delta>\<^sub>1 \<cdot> Nt X # \<delta>\<^sub>2 @ \<gamma>] # \<rho>, v @ y @ x) 
+              \<turnstile> ([X \<rightarrow> [] \<cdot> \<xi>\<^sub>1 @ Nt Y # \<xi>\<^sub>2] # ?\<sigma>, v @ y @ x)" 
             using expanding_singleton \<beta>_decomp(1) less.prems(1) by 
               (metis derive_singleton sym.inject(1), force)
           note first
           also note X_step(2)
           also from less(1)[OF \<beta>'_decomp(6) _ \<beta>'_decomp(2), of _ _ _ _ "v' @ y' @ y @ x"] 
-          have "... \<turnstile>* ([X \<rightarrow> \<xi>\<^sub>1 . Nt Y # \<xi>\<^sub>2] # ?\<sigma>, v' @ y' @ y @ x)" 
+          have "... \<turnstile>* ([X \<rightarrow> \<xi>\<^sub>1 \<cdot> Nt Y # \<xi>\<^sub>2] # ?\<sigma>, v' @ y' @ y @ x)" 
                (is "_ \<turnstile>* (?\<tau>, _)")
           using \<beta>'_decomp(5) append.assoc append_Nil X_step(1)
             by (metis \<beta>'_decomp(5) append_Nil)
-          also with Y_prod' have "... \<turnstile> ([Y \<rightarrow> [] . \<gamma>'] # ?\<tau>, v' @ y' @ y @ x)" 
+          also with Y_prod' have "... \<turnstile> ([Y \<rightarrow> [] \<cdot> \<gamma>'] # ?\<tau>, v' @ y' @ y @ x)" 
              using X_step(1) expanding by presburger
           also from less(1)[OF Y_prod(3) _ Y_prod(2), of Y "[]" "[]" _ "y' @ y @ x"]
-          have "... \<turnstile>* ([Y \<rightarrow> \<gamma>' . []] # ?\<tau>, y' @ y @ x)" 
+          have "... \<turnstile>* ([Y \<rightarrow> \<gamma>' \<cdot> []] # ?\<tau>, y' @ y @ x)" 
             using Y_prod' by simp
-          also have "... \<turnstile> ([X \<rightarrow> \<xi>\<^sub>1 @ [Nt Y] . \<xi>\<^sub>2] # ?\<sigma>, y' @ y @ x)"
+          also have "... \<turnstile> ([X \<rightarrow> \<xi>\<^sub>1 @ [Nt Y] \<cdot> \<xi>\<^sub>2] # ?\<sigma>, y' @ y @ x)"
             using reducing Y_prod' X_step(1) by presburger
           also from less(1)[OF \<beta>'_decomp(8) _ \<beta>'_decomp(4), of X _ "[]" _ "y @ x"] have
-            "... \<turnstile>* ([X \<rightarrow> \<beta>' . []] # ?\<sigma>, y @ x)"
+            "... \<turnstile>* ([X \<rightarrow> \<beta>' \<cdot> []] # ?\<sigma>, y @ x)"
             using \<beta>'_decomp(1) append.assoc X_step(1) 
             by (metis append.right_neutral append_Cons append_Nil)
           finally show ?thesis using reducing last X_step(1) \<beta>'_decomp less.prems(1) \<beta>_decomp
@@ -541,25 +541,25 @@ proof -
 qed
 
 lemma reaches_final_imp_complete_reaches_final:
-  assumes "([A \<rightarrow> \<alpha> . \<beta>] # \<rho>, w) \<turnstile>(n) ([final_state], [])"
+  assumes "([A \<rightarrow> \<alpha> \<cdot> \<beta>] # \<rho>, w) \<turnstile>(n) ([final_state], [])"
   obtains u v m k where
     "m + k = n"
     "w = u @ v"
     "Prods G' \<turnstile> \<beta> \<Rightarrow>* map Tm u"
-    "([A \<rightarrow> \<alpha> . \<beta>] # \<rho>, w) \<turnstile>(m) ([A \<rightarrow> \<alpha> @ \<beta> . []] # \<rho>, v)"
-    "([A \<rightarrow> \<alpha> @ \<beta> . []] # \<rho>, v) \<turnstile>(k) ([final_state], [])"
+    "([A \<rightarrow> \<alpha> \<cdot> \<beta>] # \<rho>, w) \<turnstile>(m) ([A \<rightarrow> \<alpha> @ \<beta> \<cdot> []] # \<rho>, v)"
+    "([A \<rightarrow> \<alpha> @ \<beta> \<cdot> []] # \<rho>, v) \<turnstile>(k) ([final_state], [])"
   using assms proof (induction n arbitrary: A \<alpha> \<beta> \<rho> w thesis rule: less_induct)
   case (less n)
   show ?case 
   proof (cases n)
     case (Suc m)
-    then obtain \<sigma> x where step: "([A \<rightarrow> \<alpha> . \<beta>] # \<rho>, w) \<turnstile> (\<sigma>, x)"
+    then obtain \<sigma> x where step: "([A \<rightarrow> \<alpha> \<cdot> \<beta>] # \<rho>, w) \<turnstile> (\<sigma>, x)"
       "(\<sigma>, x) \<turnstile>(m) ([final_state], [])"
       using less.prems(2) by (metis relpowp_Suc_D2 surj_pair)
     from step obtain B \<gamma> \<delta> \<tau> u v j k where \<sigma>_complete:
-      "\<sigma> = [B \<rightarrow> \<gamma> . \<delta>] # \<tau>" "x = u @ v" "Prods G' \<turnstile> \<delta> \<Rightarrow>* map Tm u"
-      "([B \<rightarrow> \<gamma> . \<delta>] # \<tau>, u @ v) \<turnstile>(j) ([B \<rightarrow> \<gamma> @ \<delta> . []] # \<tau>, v)"
-      "([B \<rightarrow> \<gamma> @ \<delta> . []] # \<tau>, v) \<turnstile>(k) ([final_state], [])"
+      "\<sigma> = [B \<rightarrow> \<gamma> \<cdot> \<delta>] # \<tau>" "x = u @ v" "Prods G' \<turnstile> \<delta> \<Rightarrow>* map Tm u"
+      "([B \<rightarrow> \<gamma> \<cdot> \<delta>] # \<tau>, u @ v) \<turnstile>(j) ([B \<rightarrow> \<gamma> @ \<delta> \<cdot> []] # \<tau>, v)"
+      "([B \<rightarrow> \<gamma> @ \<delta> \<cdot> []] # \<tau>, v) \<turnstile>(k) ([final_state], [])"
       "j + k = m" using less.IH 
       by (smt (verit, ccfv_SIG) Suc ipda.step_cases ipda_axioms lessI prod.inject)
     from this(5) reaches_final_imp_in_It have B_in_Prods: "(B, \<gamma> @ \<delta>) \<in> Prods G'"
@@ -569,9 +569,9 @@ lemma reaches_final_imp_complete_reaches_final:
       case (shift A' \<alpha>' a \<beta>' \<rho>' y)
       with \<sigma>_complete have eqs: "w = a # u @ v" "B = A" "\<gamma> = \<alpha> @ [Tm a]" "\<delta> = \<beta>'" by auto
       with shift have 
-        "([A \<rightarrow> \<alpha> . \<beta>] # \<rho>, w) \<turnstile> ([A \<rightarrow> \<alpha> @ [Tm a] . \<beta>'] # \<rho>, u @ v)"
+        "([A \<rightarrow> \<alpha> \<cdot> \<beta>] # \<rho>, w) \<turnstile> ([A \<rightarrow> \<alpha> @ [Tm a] \<cdot> \<beta>'] # \<rho>, u @ v)"
         using step by auto
-      also have "... \<turnstile>(j) ([A \<rightarrow> \<alpha> @ \<beta> . []] # \<rho>, v)" 
+      also have "... \<turnstile>(j) ([A \<rightarrow> \<alpha> @ \<beta> \<cdot> []] # \<rho>, v)" 
         using eqs \<sigma>_complete shift by simp
       finally show ?thesis using less.prems(1)[of "Suc j" k "a # u" v] \<sigma>_complete[unfolded eqs] Suc
         using derives_Cons shift by auto
@@ -584,36 +584,36 @@ lemma reaches_final_imp_complete_reaches_final:
       with expand step step_imp_in_Prods have Y_derives: "Prods G' \<turnstile> [Nt Y] \<Rightarrow>* map Tm u" 
         using \<sigma>_complete(3) by (metis append.right_neutral append_Nil derives_Cons_rule item.case)
       from eqs expand have exp_step:
-        "([A \<rightarrow> \<alpha> . \<beta>] # \<rho>, w) 
-          \<turnstile> ([Y \<rightarrow> [] . \<gamma>'] # [A \<rightarrow> \<alpha> . Nt Y # \<beta>'] # \<rho>, u @ v)"
+        "([A \<rightarrow> \<alpha> \<cdot> \<beta>] # \<rho>, w) 
+          \<turnstile> ([Y \<rightarrow> [] \<cdot> \<gamma>'] # [A \<rightarrow> \<alpha> \<cdot> Nt Y # \<beta>'] # \<rho>, u @ v)"
         using step by auto
       moreover with \<sigma>_complete eqs have j_steps: 
-        "... \<turnstile>(j) ([Y \<rightarrow> \<gamma>' . []] # [A \<rightarrow> \<alpha> . Nt Y # \<beta>'] # \<rho>, v)"
+        "... \<turnstile>(j) ([Y \<rightarrow> \<gamma>' \<cdot> []] # [A \<rightarrow> \<alpha> \<cdot> Nt Y # \<beta>'] # \<rho>, v)"
         using expand by simp
-      moreover have reduct_step: "... \<turnstile> ([A \<rightarrow> \<alpha> @ [Nt Y] . \<beta>'] # \<rho>, v)"
+      moreover have reduct_step: "... \<turnstile> ([A \<rightarrow> \<alpha> @ [Nt Y] \<cdot> \<beta>'] # \<rho>, v)"
         using expand step step_imp_in_Prods by force
       moreover with less.IH obtain v' x' j' k' l where complete_reaches: "v = v' @ x'" "Prods G' \<turnstile> \<beta>' \<Rightarrow>* map Tm v'"
-        "... \<turnstile>(j') ([A \<rightarrow> \<alpha> @ \<beta> . []] # \<rho>, x')"
-        "([A \<rightarrow> \<alpha> @ \<beta> . []] # \<rho>, x') \<turnstile>(k') ([final_state], [])"
+        "... \<turnstile>(j') ([A \<rightarrow> \<alpha> @ \<beta> \<cdot> []] # \<rho>, x')"
+        "([A \<rightarrow> \<alpha> @ \<beta> \<cdot> []] # \<rho>, x') \<turnstile>(k') ([final_state], [])"
         "k = Suc l"
         "j' + k' = l"
       proof - (* TODO refactor *)
         from expand step \<sigma>_complete eqs have 
-          "([Y \<rightarrow> \<gamma>' . []] # [A \<rightarrow> \<alpha> . Nt Y # \<beta>'] # \<rho>, v) 
+          "([Y \<rightarrow> \<gamma>' \<cdot> []] # [A \<rightarrow> \<alpha> \<cdot> Nt Y # \<beta>'] # \<rho>, v) 
             \<turnstile>(k) ([final_state], [])"
           by auto
-        moreover have "[Y \<rightarrow> \<gamma>' . []] # [A \<rightarrow> \<alpha> . Nt Y # \<beta>'] # \<rho> 
+        moreover have "[Y \<rightarrow> \<gamma>' \<cdot> []] # [A \<rightarrow> \<alpha> \<cdot> Nt Y # \<beta>'] # \<rho> 
           \<noteq> [final_state]"  by auto
         ultimately obtain l where l_steps: "k = Suc l"
-          "([A \<rightarrow> \<alpha> @ [Nt Y] . \<beta>'] # \<rho>, v) \<turnstile>(l) ([final_state], [])"
+          "([A \<rightarrow> \<alpha> @ [Nt Y] \<cdot> \<beta>'] # \<rho>, v) \<turnstile>(l) ([final_state], [])"
           using eqs step \<sigma>_complete reducing stepn_neq_imp_not_expanding_reaches reduct_step 
           by (metis list.sel(1) prod.inject)
         moreover with \<sigma>_complete(6) Suc have lt: "l < n" by linarith
         ultimately show thesis using less.IH[OF lt _ l_steps(2)] that expand eqs
           by (smt (verit, best) Cons_eq_append_conv append.assoc append_self_conv2)
       qed
-      ultimately have A_completes: "([A \<rightarrow> \<alpha> . \<beta>] # \<rho>, w) 
-          \<turnstile>(Suc (Suc j) + j') ([A \<rightarrow> \<alpha> @ \<beta> . []] # \<rho>, x')"
+      ultimately have A_completes: "([A \<rightarrow> \<alpha> \<cdot> \<beta>] # \<rho>, w) 
+          \<turnstile>(Suc (Suc j) + j') ([A \<rightarrow> \<alpha> @ \<beta> \<cdot> []] # \<rho>, x')"
         by (meson relpowp_Suc_I relpowp_Suc_I2 relpowp_trans)
       from complete_reaches(2) Y_derives eqs(5) have "Prods G' \<turnstile> \<beta> \<Rightarrow>* map Tm (u @ v')"
         by (metis derives_Cons_iff derives_Nt_map_TmD map_append)
@@ -626,30 +626,30 @@ qed
 
 
 lemma reaches_final_imp_completes:
-  assumes "([A \<rightarrow> \<alpha> . \<beta>] # \<rho>, w) \<turnstile>* ([final_state], [])"
+  assumes "([A \<rightarrow> \<alpha> \<cdot> \<beta>] # \<rho>, w) \<turnstile>* ([final_state], [])"
   obtains u v where 
     "w = u @ v"
     "Prods G' \<turnstile> \<beta> \<Rightarrow>* map Tm u"
-    "([A \<rightarrow> \<alpha> . \<beta>] # \<rho>, w) \<turnstile>* ([A \<rightarrow> \<alpha> @ \<beta> . []] # \<rho>, v)"
-    "([A \<rightarrow> \<alpha> @ \<beta> . []] # \<rho>, v) \<turnstile>* ([final_state], [])"
+    "([A \<rightarrow> \<alpha> \<cdot> \<beta>] # \<rho>, w) \<turnstile>* ([A \<rightarrow> \<alpha> @ \<beta> \<cdot> []] # \<rho>, v)"
+    "([A \<rightarrow> \<alpha> @ \<beta> \<cdot> []] # \<rho>, v) \<turnstile>* ([final_state], [])"
 proof -
   from assms have A_in_Prods: "(A, \<alpha> @ \<beta>) \<in> Prods G'" 
     using reaches_final_imp_in_It in_It_imp_in_Prods by fastforce
   from reaches_final_imp_complete_reaches_final assms rtranclp_imp_relpowp obtain u v where complete:
     "w = u @ v"
     "Prods G' \<turnstile> \<beta> \<Rightarrow>* map Tm u"
-    "([A \<rightarrow> \<alpha> @ \<beta> . []] # \<rho>, v) \<turnstile>* ([final_state], [])" 
+    "([A \<rightarrow> \<alpha> @ \<beta> \<cdot> []] # \<rho>, v) \<turnstile>* ([final_state], [])" 
     using relpowp_imp_rtranclp by metis
   with derives_imp_completes[OF this(2), of A \<alpha> "[]"] A_in_Prods show thesis using that
     by simp
 qed
 
 lemma reaches_final_imp_second_is_chain:
-  assumes "([A \<rightarrow> \<alpha> . \<beta>] # i # \<rho>, w) \<turnstile>* ([final_state], [])"
-  obtains X \<alpha>' \<beta>' where "i = [X \<rightarrow> \<alpha>' . Nt A # \<beta>']"
+  assumes "([A \<rightarrow> \<alpha> \<cdot> \<beta>] # i # \<rho>, w) \<turnstile>* ([final_state], [])"
+  obtains X \<alpha>' \<beta>' where "i = [X \<rightarrow> \<alpha>' \<cdot> Nt A # \<beta>']"
 proof -
   from assms reaches_final_imp_completes obtain x where 
-    "([A \<rightarrow> \<alpha> @ \<beta> . []] # i # \<rho>, x) \<turnstile>* ([final_state], [])"
+    "([A \<rightarrow> \<alpha> @ \<beta> \<cdot> []] # i # \<rho>, x) \<turnstile>* ([final_state], [])"
     by metis
   then show thesis
   proof (cases rule: converse_rtranclpE)
@@ -660,13 +660,13 @@ proof -
 qed
 
 lemma reaches_without_stack_imp_S':
-  assumes "([[A \<rightarrow> \<alpha> . \<beta>]], w) \<turnstile>* ([final_state], [])"
-  shows "[A \<rightarrow> \<alpha> . \<beta>] = init M \<or> [A \<rightarrow> \<alpha> . \<beta>] = final_state"
+  assumes "([[A \<rightarrow> \<alpha> \<cdot> \<beta>]], w) \<turnstile>* ([final_state], [])"
+  shows "[A \<rightarrow> \<alpha> \<cdot> \<beta>] = init M \<or> [A \<rightarrow> \<alpha> \<cdot> \<beta>] = final_state"
 proof -
   from reaches_final_imp_completes[of _ _ _ "[]"] assms obtain u v where "w = u @ v"
     "Prods G' \<turnstile> \<beta> \<Rightarrow>* map Tm u"
-    "([[A \<rightarrow> \<alpha> . \<beta>]], w) \<turnstile>* ([[A \<rightarrow> \<alpha> @ \<beta> . []]], v)"
-    "([[A \<rightarrow> \<alpha> @ \<beta> . []]], v) \<turnstile>* ([final_state], [])"
+    "([[A \<rightarrow> \<alpha> \<cdot> \<beta>]], w) \<turnstile>* ([[A \<rightarrow> \<alpha> @ \<beta> \<cdot> []]], v)"
+    "([[A \<rightarrow> \<alpha> @ \<beta> \<cdot> []]], v) \<turnstile>* ([final_state], [])"
     (is "?complete \<turnstile>* ?final")
     by metis
   from this(4) have "?complete = ?final"
@@ -741,7 +741,7 @@ lemma deriver_imp_IPDA_comp:
     "Prods G' \<turnstile> [Nt S'] \<Rightarrow>r \<alpha>@\<beta>"
     "Prods G' \<turnstile> \<beta> \<Rightarrow>* map Tm v"
   shows
-    "([[S' \<rightarrow> \<alpha> . \<beta>]], v) \<turnstile>* ([final_state], [])"
+    "([[S' \<rightarrow> \<alpha> \<cdot> \<beta>]], v) \<turnstile>* ([final_state], [])"
 proof -
   from assms have eq_S: "\<alpha>@\<beta> = [Nt S]" 
     using S'_derive_imp_S append_eq_Cons_conv 
